AP/AP.lean
@@ -1,1 +1,1 @@
-import AP.AP.Basic
+import AP.AP.Determinacy
