AP/AP/Determinacy.lean
@@ -1,0 +1,89 @@
+import AP.AP.Basic
+
+namespace AP
+
+theorem State.not_a_hws_of_d_hws {s : State} (h : s.d_hws) : ¬s.a_hws := by
+  obtain ⟨d, hd, h⟩ := h
+  simp [a_hws]
+  intro a ha
+  use d, hd
+  exact h a ha
+
+def aOptimalCnd (sa : State) (pa : PointZ) : Prop :=
+  ∃ sd, sys.tr sa pa = some sd ∧ ∀ pd sa', sys.tr sd pd = some sa' → sa'.a_hws
+
+open Classical in noncomputable
+def aOptimal : AStrat :=
+  .mk # λ sa => if ∃ pa, aOptimalCnd sa pa
+  then Classical.epsilon # aOptimalCnd sa
+  else Classical.epsilon # sys.validTr sa
+
+theorem wf_aOptimal : aOptimal.WF := by
+  rw [aStrat_wf_iff]
+  intro sa hsa h₁
+  dsimp [aOptimal]
+  generalize hp : Classical.epsilon (aOptimalCnd sa) = pa
+  simp
+  split_ifs with h₂
+  rotate_left
+  · have h₃ := Classical.epsilon_spec h₁
+    simp at h₃
+    exact h₃
+  simp at h₁
+  have h₃ := Classical.epsilon_spec h₂
+  rw [hp] at h₃
+  simp [aOptimalCnd] at h₃
+  exact h₃.1
+
+instance : aOptimal.WF := wf_aOptimal
+
+-- #check 0 #exit
+
+theorem AState.of_ind {sa sa'} [hs : AState sa] [hs' : AState sa] {p : State → Prop}
+(h₁ : p sa) (h₂ : ∀ sa [AState sa] pa sd pd sa',
+sys.tr sa pa = some sd → sys.tr sd pd = some sa' → p sa')
+(h₃ : sys.Reachable sa sa') : p sa' := by
+  sorry
+
+-- #check 0 #exit
+
+theorem AState.a_hws_of_ind {sa : State} [hs : AState sa] {p : State → Prop}
+(h₁ : p sa) (h₂ : ∀ sa [AState sa], p sa → ∃ pa sd, sys.tr sa pa = some sd ∧
+∀ pd sa', sys.tr sd pd = some sa' → p sa') : sa.a_hws := by
+  classical
+  use aOptimal, inferInstance
+  intro d hd
+  intro n
+  induction n generalizing sa p; simp
+  nm n ih
+  have h₄ := ih h₁ h₂
+  rw [System.simulate_add]
+  simp [h₄]
+  generalize h₃ : sys.simulate (Strat.mk aOptimal d).f sa n = r at h₄ ⊢
+  rcases r with ⟨sa', r⟩
+  dsimp at h₄ ⊢
+  subst h₄
+  sorry
+
+#check 0 #exit
+
+theorem State.a_hws_of_ind {s : State} [hs : s.WF] {p : State → Prop}
+(h₁ : p s)
+(h₂ : ∀ s [s.WF], )
+
+#check 0 #exit
+
+theorem State.a_hws_of_not_d_hws {s : State} [hs : s.WF] (h : ¬s.d_hws) : s.a_hws := by
+  simp [d_hws] at h
+  simp [a_hws]
+
+#check 0 #exit
+
+@[simp]
+theorem State.not_a_hws_iff {s : State} [hs : s.WF] : ¬s.a_hws ↔ s.d_hws := by
+  refine' ⟨λ h => _, s.not_a_hws_of_d_hws⟩
+  contrapose! h; exact s.a_hws_of_not_d_hws h
+
+@[simp]
+theorem State.not_d_hws_iff_a_hws {s : State} [hs : s.WF] : ¬s.d_hws ↔ s.a_hws := by
+  simp [not_iff_comm']
